

**The University of Hong Kong**  
**Department of Statistics and Actuarial Science**

**STAT 6015/6115/7615 Advanced Quantitative Risk Management and Finance**

**Solution for Assignment 2**

1. Let  $a = \text{var}(X)$ ,  $b = \text{var}(W)$  and  $c = \text{cov}(X, W)$ . Then

$$f(\alpha) := \text{var}(\alpha X + (1 - \alpha)W) = \alpha^2 a + (1 - \alpha)^2 b + 2\alpha(1 - \alpha)c$$

and by setting  $f'(\alpha) = 0$ ,  $\alpha = \frac{b-c}{a+b-2c}$ . It can be checked that  $f''(\alpha) \geq 0$ . The minimum variance is  $\frac{ab-c^2}{a+b-2c}$ . When  $X$  and  $W$  are independent, the minimum variance is  $\frac{ab}{a+b}$  and  $\alpha = \frac{b}{a+b}$ .

2. Denote  $S_t = S_0 e^{Y_t}$ , where  $Y_t = (r - \sigma^2/2)t + \sigma W_t$ . So we have

$$\left( \prod_{i=1}^k S_{\frac{iT}{k}} \right)^{1/k} = S_0 \exp \left( \frac{1}{k} \sum_{i=1}^k Y_{\frac{iT}{k}} \right) = S_0 e^{\bar{Y}},$$

where  $\bar{Y} = \frac{1}{k} \sum_{i=1}^k Y_{\frac{iT}{k}}$  and  $Y_{\frac{iT}{k}} = \left( r - \frac{\sigma^2}{2} \right) \frac{iT}{k} + \sigma W_{\frac{iT}{k}}$ . By letting  $Y_0 = 0$ ,  $\bar{Y}$  can be written as

$$\begin{aligned} \bar{Y} &= \frac{1}{k} \sum_{i=1}^k Y_{\frac{iT}{k}} = \frac{1}{k} \sum_{i=1}^k (k - i + 1) \left( Y_{\frac{iT}{k}} - Y_{\frac{(i-1)T}{k}} \right) \\ &= \frac{1}{k} \sum_{i=1}^k (k - i + 1) \left[ \left( r - \frac{\sigma^2}{2} \right) \frac{T}{k} + \sigma \left( W_{\frac{iT}{k}} - W_{\frac{(i-1)T}{k}} \right) \right] \\ &= \frac{1}{k} \sum_{i=1}^k (k - i + 1) \left[ \left( r - \frac{\sigma^2}{2} \right) \frac{T}{k} + \sigma \sqrt{\frac{T}{k}} Z_i \right], \end{aligned}$$

where  $Z_i = W_i - W_{i-1} \stackrel{\text{i.i.d.}}{\sim} N(0, 1)$ . Therefore,  $\bar{Y}$  is normally distributed with mean

$$\begin{aligned} E(\bar{Y}) &= \frac{1}{k} \sum_{i=1}^k (k - i + 1) \left[ \left( r - \frac{\sigma^2}{2} \right) \frac{T}{k} + \sigma \sqrt{\frac{T}{k}} E(Z_i) \right] \\ &= \frac{1}{k} \sum_{i=1}^k (k - i + 1) \left[ \left( r - \frac{\sigma^2}{2} \right) \frac{T}{k} \right] \\ &= \left( r - \frac{\sigma^2}{2} \right) \frac{T}{k} \frac{1}{k} \sum_{i=1}^k i \\ &= \left( r - \frac{\sigma^2}{2} \right) \frac{T}{k} \frac{1}{k} \left[ \frac{1}{2} k(k+1) \right] \\ &= \frac{1}{2} \left( r - \frac{\sigma^2}{2} \right) \left( 1 + \frac{1}{k} \right) T \end{aligned}$$

and variance

$$\begin{aligned}
\text{Var}(\bar{Y}) &= \frac{1}{k^2} \sum_{i=1}^k (k-i+1)^2 \sigma^2 \frac{T}{k} \\
&= \sigma^2 \frac{T}{k} \frac{1}{k^2} \sum_{i=1}^k i^2 \\
&= \sigma^2 \frac{T}{k} \frac{1}{k^2} \left[ \frac{1}{3} k \left( k + \frac{1}{2} \right) (k+1) \right] \\
&= \frac{\sigma^2}{3} \left( 1 + \frac{1}{k} \right) \left( 1 + \frac{1}{2k} \right) T.
\end{aligned}$$

That is,  $\bar{Y} \sim N(\tilde{\mu}T, \tilde{\sigma}^2 T)$ , where

$$\tilde{\mu} = \frac{1}{2} \left( r - \frac{\sigma^2}{2} \right) \left( 1 + \frac{1}{k} \right), \quad \tilde{\sigma}^2 = \frac{\sigma^2}{3} \left( 1 + \frac{1}{k} \right) \left( 1 + \frac{1}{2k} \right).$$

3. Note that  $f(x) = \frac{1}{\sqrt{2\pi\sigma^2}} e^{-\frac{(x-\mu)^2}{2\sigma^2}}$ . Then the tilted density is

$$\begin{aligned}
f_t(x) &= \left( \int e^{ty} f(y) dy \right)^{-1} e^{tx} f(x) \\
&= e^{-\frac{1}{2\sigma^2}(-2\mu\sigma^2 t + \sigma^4 t^2)} e^{tx} \frac{1}{\sqrt{2\pi\sigma^2}} e^{-\frac{(x-\mu)^2}{2\sigma^2}} \\
&= \frac{1}{\sqrt{2\pi\sigma^2}} e^{-\frac{(x-\mu-\sigma^2 t)^2}{2\sigma^2}} \sim N(\mu + \sigma^2 t, \sigma^2).
\end{aligned}$$

4. Let  $h$  be a bounded measurable function, then

$$\begin{aligned}
E_{\mathbb{Q}}(h(X)) &= \int_{\Omega} h(X(\omega)) d\mathbb{Q}(\omega) = \int_{\Omega} h(X(\omega)) \frac{d\mathbb{Q}}{d\mathbb{P}}(\omega) d\mathbb{P}(\omega) \\
&= \int_{\Omega} h(X(\omega)) \frac{g(X(\omega))}{f(X(\omega))} d\mathbb{P}(\omega) = E_{\mathbb{P}}(h(X) \frac{g(X)}{f(X)}) \\
&= \int_{\mathbb{R}} h(x) \frac{g(x)}{f(x)} f(x) dx = \int_{\mathbb{R}} h(x) g(x) dx.
\end{aligned}$$

5. For the crude Monte Carlo estimator, the variance is

$$\begin{aligned}
\sigma_c^2 &= \frac{1}{2n} \text{Var} \left( \frac{e^{U_i} - 1}{e - 1} \right) = \frac{1}{2n(e-1)^2} \text{Var}(e^{U_i}) = \frac{1}{2n(e-1)^2} \{E(e^{2U_i}) - [E(e^{U_i})]^2\} \\
&= \frac{1}{2n(e-1)^2} \left[ \frac{e^2 - 1}{2} - (e-1)^2 \right] = \frac{3-e}{4n(e-1)} = \frac{0.04099}{n}.
\end{aligned}$$

For the antithetic variable method, the Monte Carlo estimator is

$$\hat{\theta}_a = \frac{1}{2n} \sum_{i=1}^n \left( \frac{e^{U_i} - 1}{e - 1} + \frac{e^{1-U_i} - 1}{e - 1} \right).$$

The variance of this estimator is

$$\begin{aligned}
\sigma_a^2 &= \frac{1}{n} \text{Var} \left( \frac{e^{U_i} - 1}{2(e-1)} + \frac{e^{1-U_i} - 1}{2(e-1)} \right) = \frac{1}{4n(e-1)^2} \text{Var}(e^{U_i} + e^{1-U_i}) \\
&= \frac{1}{4n(e-1)^2} [\text{Var}(e^{U_i}) + \text{Var}(e^{1-U_i}) + 2\text{Cov}(e^{U_i}, e^{1-U_i})] \\
&= \frac{1}{4n(e-1)^2} \{2\text{Var}(e^{U_i}) + 2[E(e^{U_i}e^{1-U_i}) - E(e^{U_i})E(e^{1-U_i})]\} \\
&= \frac{1}{2n(e-1)^2} \left[ \frac{(e-1)(3-e)}{2} + e - (e-1)^2 \right] = \frac{0.001325}{n}.
\end{aligned}$$

So the efficiency of this estimator relative to the crude Monte Carlo estimator is

$$\frac{\sigma_c^2}{\sigma_a^2} = \frac{0.04099/n}{0.001325/n} = 30.9311.$$